examples/Smram.v
@@ -1,0 +1,78 @@
+Require Import Coq.Bool.Sumbool.
+
+Require Import FreeSpec.Interp.
+Require Import FreeSpec.Compose.
+Require Import FreeSpec.Refine.
+Require Import FreeSpec.Program.
+
+Require Import FreeSpec.Examples.Map.
+
+Section SMRAM_EXAMPLE.
+  Variables (Addr: Type)
+            (Value: Type)
+            (Smram: Addr -> Prop)
+            (Smramdec: forall (a: Addr), {Smram a}+{~Smram a}).
+
+  Inductive IMCH
+    : Interface :=
+  | ReadMem (a: Addr)
+            (smm: bool)
+    : IMCH Value
+  | WriteMem (a: Addr)
+             (v: Value)
+             (smm: bool)
+    : IMCH unit.
+
+  Record MCH
+    : Type :=
+    { smram_lock: bool
+    }.
+
+  Definition IDRAM := IMap Addr Value.
+  Definition IVGA := IMap Addr Value.
+
+  Local Open Scope prog_scope.
+
+  Definition read_dram
+             (a: Addr)
+    : Program (IDRAM <+> IVGA) Value :=
+    [ileft (Read _ _ a)].
+
+  Definition read_vga
+             (a: Addr)
+    : Program (IDRAM <+> IVGA) Value :=
+    [iright (Read _ _ a)].
+
+  Definition write_dram
+             (a: Addr)
+             (v: Value)
+    : Program (IDRAM <+> IVGA) unit :=
+    [ileft (Write _ _ a v)].
+
+  Definition write_vga
+             (a: Addr)
+             (v: Value)
+    : Program (IDRAM <+> IVGA) unit :=
+    [iright (Write _ _ a v)].
+
+  Program Definition mch_refine
+    : StatefulRefinement IMCH (IDRAM <+> IVGA) MCH :=
+    fun {A: Type} (i: IMCH A) (s: MCH) =>
+      match i with
+      | ReadMem a true => x <- read_dram a
+                        ; ret (x, s)
+      | ReadMem a false => x <- if andb (bool_of_sumbool (Smramdec a))
+                                        (smram_lock s)
+                                then read_vga a
+                                else read_dram a
+                         ; ret (x, s)
+
+      | WriteMem a v true => write_dram a v
+                          ;; ret (tt, s)
+      | WriteMem a v false => (if andb (bool_of_sumbool (Smramdec a))
+                                       (smram_lock s)
+                              then write_vga a v
+                              else write_dram a v)
+                           ;; ret (tt, s)
+      end.
+End SMRAM_EXAMPLE.
